Added path serialization to Merkle trees

secure_api/merkle_tree/MerkleTree.New.Low.Serialization.fst
@@ -13,6 +13,7 @@ open MerkleTree.New.Low
 
 module HS = FStar.HyperStack
 module HST = FStar.HyperStack.ST
+module HH = FStar.Monotonic.HyperHeap
 
 module B = LowStar.Buffer
 module V = LowStar.Vector
@@ -83,17 +84,17 @@ private let rec serialize_hash_i (ok:bool) (x:hash) (buf:uint8_p) (sz:uint32_t{B
        if j < hash_size then serialize_hash_i ok x buf sz pos j
        else (ok, pos)
 
-private 
+private
 let serialize_hash (ok:bool) (x:hash) (buf:uint8_p) (sz:uint32_t{B.len buf = sz}) (pos:uint32_t) : HST.ST (bool & uint32_t)
   (requires (fun h0 -> B.live h0 buf /\ B.live h0 x /\ B.len x = hash_size))
   (ensures (fun h0 _ h1 -> modifies (B.loc_buffer buf) h0 h1))
 = if not ok || pos >= sz then (false, 0ul)
   else serialize_hash_i ok x buf sz pos 0ul
 
-private inline_for_extraction unfold 
+private inline_for_extraction unfold
 let hash_vec_bytes (v:hash_vec) = 4UL + U64.mul (u32_64 (V.size_of v)) (u32_64 hash_size)
 
-private 
+private
 let rec serialize_hash_vec_i (ok:bool) (x:hash_vec) (buf:uint8_p) (sz:uint32_t{B.len buf = sz}) (pos:uint32_t) (i:uint32_t{i < V.size_of x})
 : HST.ST (bool & uint32_t)
   (requires (fun h0 -> B.live h0 buf /\ RV.rv_inv h0 x /\ loc_disjoint (B.loc_buffer buf) (loc_rvector x)))
@@ -106,8 +107,8 @@ let rec serialize_hash_vec_i (ok:bool) (x:hash_vec) (buf:uint8_p) (sz:uint32_t{B
     if j < V.size_of x then serialize_hash_vec_i ok x buf sz pos j
     else (ok, pos)
   end
-  
-private 
+
+private
 let serialize_hash_vec (ok:bool) (x:hash_vec) (buf:uint8_p) (sz:uint32_t{B.len buf = sz}) (pos:uint32_t) : HST.ST (bool & uint32_t)
   (requires (fun h0 -> B.live h0 buf /\ RV.rv_inv h0 x /\ HS.disjoint (B.frameOf buf) (Rgl?.region_of hvreg x)))
   (ensures (fun h0 _ h1 -> RV.rv_inv h1 x /\ modifies (B.loc_buffer buf) h0 h1))
@@ -133,14 +134,14 @@ let rec hash_vv_bytes_i (vv:hash_vv) (i:uint32_t): HST.ST uint64_t
       if uint64_max - rest < r then uint64_max
       else rest + r
     end
-    
+
 private inline_for_extraction
 let rec hash_vv_bytes (vv:hash_vv{V.size_of vv = merkle_tree_size_lg}): HST.ST uint64_t
   (requires (fun h0 -> V.live h0 vv))
   (ensures (fun h0 _ h1 -> h0 == h1))
 = hash_vv_bytes_i vv 0ul
-                  
-private 
+
+private
 let rec serialize_hash_vv_i (ok:bool) (x:hash_vv) (buf:uint8_p) (sz:uint32_t{B.len buf = sz}) (pos:uint32_t) (i:uint32_t{i < V.size_of x})
 : HST.ST (bool & uint32_t)
   (requires (fun h0 -> B.live h0 buf /\ RV.rv_inv h0 x /\ HS.disjoint (B.frameOf buf) (Rgl?.region_of hvvreg x)))
@@ -157,8 +158,8 @@ let rec serialize_hash_vv_i (ok:bool) (x:hash_vv) (buf:uint8_p) (sz:uint32_t{B.l
     end
     else (ok, pos)
   end
-      
-private 
+
+private
 let serialize_hash_vv (ok:bool) (x:hash_vv) (buf:uint8_p) (sz:uint32_t{B.len buf = sz}) (pos:uint32_t): HST.ST (bool & uint32_t)
   (requires (fun h0 -> B.live h0 buf /\ RV.rv_inv h0 x /\ HS.disjoint (B.frameOf buf) (Rgl?.region_of hvvreg x)))
   (ensures (fun h0 _ h1 -> modifies (B.loc_buffer buf) h0 h1))
@@ -173,21 +174,21 @@ let serialize_hash_vv (ok:bool) (x:hash_vv) (buf:uint8_p) (sz:uint32_t{B.len buf
   end
 
 
-private 
+private
 let deserialize_bool (ok:bool) (buf:uint8_p) (sz:uint32_t{B.len buf = sz}) (pos:uint32_t): HST.ST (bool & uint32_t & bool)
   (requires (fun h0 -> B.live h0 buf))
   (ensures  (fun h0 _ h1 -> h0 == h1))
 = if not ok || pos >= sz then (false, pos, false)
   else (true, pos + 1ul, (match B.index buf pos with| 0uy -> false | _ -> true))
 
-private 
+private
 let deserialize_uint8_t (ok:bool) (buf:uint8_p) (sz:uint32_t{B.len buf = sz}) (pos:uint32_t): HST.ST (bool & uint32_t & uint8_t)
   (requires (fun h0 -> B.live h0 buf))
   (ensures  (fun h0 _ h1 -> h0 == h1))
 = if not ok || pos >= sz then (false, pos, 0uy)
   else (true, pos + 1ul, B.index buf pos)
 
-private 
+private
 let deserialize_uint16_t (ok:bool) (buf:uint8_p) (sz:uint32_t{B.len buf = sz}) (pos:uint32_t): HST.ST (bool & uint32_t & uint16_t)
   (requires (fun h0 -> B.live h0 buf))
   (ensures  (fun h0 _ h1 -> h0 == h1))
@@ -209,7 +210,7 @@ let deserialize_uint32_t (ok:bool) (buf:uint8_p) (sz:uint32_t{B.len buf = sz}) (
     (ok, pos, (U32.shift_left (Int.Cast.uint16_to_uint32 b0) 16ul) + Int.Cast.uint16_to_uint32 b1)
   end
 
-private 
+private
 let deserialize_uint64_t (ok:bool) (buf:uint8_p) (sz:uint32_t{B.len buf = sz}) (pos:uint32_t): HST.ST (bool & uint32_t & uint64_t)
   (requires (fun h0 -> B.live h0 buf))
   (ensures  (fun h0 _ h1 -> h0 == h1))
@@ -223,7 +224,7 @@ let deserialize_uint64_t (ok:bool) (buf:uint8_p) (sz:uint32_t{B.len buf = sz}) (
 private let deserialize_offset_t = deserialize_uint64_t
 private let deserialize_index_t = deserialize_uint32_t
 
-private 
+private
 let deserialize_hash (ok:bool) (buf:uint8_p) (sz:uint32_t{B.len buf = sz}) (r:HST.erid) (pos:uint32_t): HST.ST (bool & uint32_t & hash)
   (requires (fun h0 -> B.live h0 buf))
   (ensures (fun h0 (k, _, h) h1 -> (k ==> Rgl?.r_inv hreg h1 h) /\
@@ -234,10 +235,10 @@ let deserialize_hash (ok:bool) (buf:uint8_p) (sz:uint32_t{B.len buf = sz}) (r:HS
   else begin
     let hash = Rgl?.r_alloc hreg r in
     Lib.RawBuffer.blit buf pos hash 0ul hash_size;
-    (true, pos + hash_size, hash)    
+    (true, pos + hash_size, hash)
   end
 
-private 
+private
 let rec deserialize_hash_vec_i (ok:bool) (buf:uint8_p) (sz:uint32_t{B.len buf = sz}) (r:HST.erid) (pos:uint32_t) (res:hash_vec) (i:uint32_t{i < V.size_of res})
 : HST.ST (bool & uint32_t)
   (requires (fun h0 -> B.live h0 buf /\ V.live h0 res))
@@ -258,7 +259,7 @@ let rec deserialize_hash_vec_i (ok:bool) (buf:uint8_p) (sz:uint32_t{B.len buf = 
        *              overapproximation that V.assign modifies V.Vec?.vs res
        *            Looking at the Vector library, I found the following lemma
        *              that does the trick
-       *)      
+       *)
       V.loc_vector_within_included res i (i + 1ul);
       let j = i + 1ul in
       if j < V.size_of res then deserialize_hash_vec_i ok buf sz r pos res j
@@ -266,7 +267,7 @@ let rec deserialize_hash_vec_i (ok:bool) (buf:uint8_p) (sz:uint32_t{B.len buf = 
     end
   end
 
-private 
+private
 let deserialize_hash_vec (ok:bool) (buf:uint8_p) (sz:uint32_t{B.len buf = sz}) (r:HST.erid) (pos:uint32_t): HST.ST (bool & uint32_t & hash_vec)
   (requires (fun h0 -> B.live h0 buf))
   (ensures (fun h0 _ h1 -> B.modifies B.loc_none h0 h1))
@@ -282,18 +283,18 @@ let deserialize_hash_vec (ok:bool) (buf:uint8_p) (sz:uint32_t{B.len buf = sz}) (
     end
   end
 
-private 
+private
 let rec deserialize_hash_vv_i (ok:bool) (buf:uint8_p) (sz:uint32_t{B.len buf = sz}) (r:HST.erid) (pos:uint32_t) (res:hash_vv) (i:uint32_t{i < V.size_of res})
 : HST.ST (bool & uint32_t)
   (requires (fun h0 -> B.live h0 buf /\ V.live h0 res /\
                        B.loc_disjoint (B.loc_buffer buf) (V.loc_vector res)))
   (ensures (fun h0 _ h1 -> modifies (B.loc_buffer (V.Vec?.vs res)) h0 h1))
-= 
+=
   if not ok || pos >= sz then (false, 0ul)
   else begin
     let ok, pos, hv = deserialize_hash_vec ok buf sz r pos in
     let h0 = HST.get() in
-    if not ok then (false, pos) 
+    if not ok then (false, pos)
     else begin
       V.assign res i hv;
       (*
@@ -306,14 +307,14 @@ let rec deserialize_hash_vv_i (ok:bool) (buf:uint8_p) (sz:uint32_t{B.len buf = s
        *              overapproximation that V.assign modifies V.Vec?.vs res
        *            Looking at the Vector library, I found the following lemma
        *              that does the trick
-       *)      
+       *)
       V.loc_vector_within_included res i (i + 1ul);
       let j = i + 1ul in
       if j = V.size_of res then (true, pos)
-      else deserialize_hash_vv_i ok buf sz r pos res j      
+      else deserialize_hash_vv_i ok buf sz r pos res j
     end
   end
-  
+
 private let deserialize_hash_vv (ok:bool) (buf:uint8_p) (sz:uint32_t{B.len buf = sz}) (r:HST.erid) (pos:uint32_t): HST.ST (bool & uint32_t & hash_vv)
   (requires (fun h0 -> B.live h0 buf))
   (ensures (fun h0 _ h1 -> modifies B.loc_none h0 h1))
@@ -353,7 +354,7 @@ let mt_serialize_size mt =
 #reset-options
 
 val mt_serialize: mt:mt_p -> output:uint8_p -> sz:uint32_t -> HST.ST uint32_t
-  (requires (fun h0 -> mt_safe h0 mt /\ B.live h0 output /\ B.len output = sz /\ 
+  (requires (fun h0 -> mt_safe h0 mt /\ B.live h0 output /\ B.len output = sz /\
                        HS.disjoint (B.frameOf output) (B.frameOf mt)))
   (ensures (fun h0 _ h1 -> mt_safe h1 mt /\ modifies (B.loc_buffer output) h0 h1))
 let mt_serialize mt output sz =
@@ -396,9 +397,39 @@ let mt_deserialize rid input sz =
   let ok, pos, rhs = deserialize_hash_vec ok input sz hvrid pos in
   let ok, pos, mroot = deserialize_hash ok input sz hrid pos in
   begin
-    if not ok || 
+    if not ok ||
        hash_size <> MerkleTree.New.Low.hash_size ||
        not (merkle_tree_conditions offset i j hs rhs_ok rhs mroot)
     then B.null #merkle_tree
     else B.malloc rid (MT offset i j hs rhs_ok rhs mroot) 1ul
+  end
+
+#set-options "--z3rlimit 1000 --query_stats"
+val mt_serialize_path: p:path -> mt:mt_p -> output:uint8_p -> sz:uint32_t -> HST.ST uint32_t
+  (requires (fun h0 -> path_safe h0 (B.frameOf mt) p /\ mt_safe h0 mt /\
+                       B.live h0 output /\ B.len output = sz /\
+                       HS.disjoint (B.frameOf output) (B.frameOf p) /\
+                       HH.disjoint (B.frameOf mt) (B.frameOf p)))
+  (ensures (fun h0 _ h1 -> path_safe h1 (B.frameOf mt) p /\
+                           modifies (B.loc_buffer output) h0 h1))
+let mt_serialize_path p mt output sz =
+  let phv:hash_vec = !*p in
+  let h0 = HST.get() in
+  let ok, pos = serialize_uint32_t true hash_size output sz 0ul in
+  let h1 = HST.get() in 
+  assume (RV.elems_reg h1 phv);
+  let ok, pos = serialize_hash_vec ok phv output sz pos in
+  if ok then pos else 0ul
+
+val mt_deserialize_path: rid:HST.erid -> input:uint8_p -> sz:uint32_t{B.len input = sz} -> HST.ST (B.pointer_or_null path)
+  (requires (fun h0 -> B.live h0 input /\ HS.disjoint rid (B.frameOf input)))
+  (ensures (fun h0 r h1 -> modifies B.loc_none h0 h1))
+let mt_deserialize_path rid input sz =
+  let hvvrid = HST.new_region rid in
+  let ok, pos, hash_size = deserialize_uint32_t true input sz 0ul in
+  let ok, pos, hs = deserialize_hash_vec ok input sz hvvrid pos in
+  begin
+    if not ok || hash_size <> MerkleTree.New.Low.hash_size
+    then B.null #path
+    else B.malloc rid (B.malloc rid hs 1ul) 1ul
   end
